rpc/impl.v
@@ -11,42 +11,42 @@ Set Implicit Arguments.
 Unset Strict Implicit.
 Unset Printing Implicit Defensive.
 
+Notation rpcN := (nroot.@"rpc").
+
 Module Impl.
 
 Section Impl.
 
-Variable N : namespace.
-
 Definition connect : val := λ: "c" "skA" "vkB",
-  Conn.connect (N.@"rpc".@"auth") "c" "skA" "vkB".
+  Conn.connect "c" "skA" "vkB".
 
 Definition listen : val := λ: "c", Conn.listen "c".
 
 Definition confirm : val := λ: "c" "skB" "req",
-  Conn.confirm (N.@"rpc".@"auth") "c" "skB" "req".
+  Conn.confirm "c" "skB" "req".
 
-Definition call (s : string) : val := λ: "c" "cs" "ts",
+Definition call N (s : string) : val := λ: "c" "cs" "ts",
   Conn.write "c" "cs" (Tag $ N.@s.@"call") "ts";;
   Conn.read "c" "cs" (Tag $ N.@s.@"resp").
 
-Definition handle (s : string) : val := λ: "c" "f",
+Definition handle N (s : string) : val := λ: "c" "f",
   Conn.handle (Tag $ N.@s.@"call")
     (λ: "cs" "ts",
       match: "f" "ts" with
         SOME "res" => Conn.write "c" "cs" (Tag (N.@s.@"resp")) "res"
-      | NONE => Conn.write "c" "cs" (Tag (N.@"rpc".@"error")) [TInt 0]
+      | NONE => Conn.write "c" "cs" (Tag (rpcN.@"error")) [TInt 0]
       end;;
       #true).
 
 Definition close : val := λ: "c" "cs",
-  Conn.write "c" "cs" (Tag $ N.@"rpc".@"close".@"call") [TInt 0];;
-  Conn.read  "c" "cs" (Tag $ N.@"rpc".@"close".@"resp");;
+  Conn.write "c" "cs" (Tag $ rpcN.@"close".@"call") [TInt 0];;
+  Conn.read  "c" "cs" (Tag $ rpcN.@"close".@"resp");;
   Conn.free "c" "cs".
 
 Definition handle_close : val := λ: "c",
-  Conn.handle (Tag $ N.@"rpc".@"close".@"call")
+  Conn.handle (Tag $ rpcN.@"close".@"call")
     (λ: "cs" "ts",
-      Conn.write "c" "cs" (Tag (N.@"rpc".@"close".@"resp")) [TInt 0];;
+      Conn.write "c" "cs" (Tag (rpcN.@"close".@"resp")) [TInt 0];;
       Conn.free "c" "cs";;
       #false).
 
