store/shared.v
@@ -16,6 +16,8 @@ Unset Printing Implicit Defensive.
 
 Local Existing Instance ticket_lock.
 
+Notation dbN := (nroot.@"db").
+
 Record server_state := {
   ss_key : term;
   ss_clients : val;
@@ -67,22 +69,20 @@ Implicit Types b : bool.
 Implicit Types v : val.
 Implicit Types (failed : bool).
 
-Variable N : namespace.
-
 Definition db_client_ready kI kR db : iProp :=
   ∃ os, ⌜db = DB.to_db os⌝ ∗
-        rep_main kI kR N os ∗ rep_current kI kR N [] os.
+        rep_main kI kR dbN os ∗ rep_current kI kR dbN [] os.
 
 Definition db_server_ready kI kR db : iProp :=
-  ∃ os, ⌜db = DB.to_db os⌝ ∗ rep_copy kI kR N [] os.
+  ∃ os, ⌜db = DB.to_db os⌝ ∗ rep_copy kI kR dbN [] os.
 
 Definition db_disconnected kI kR : iProp := ∃ db,
   (Conn.failure kI kR ∨ db_client_ready kI kR db) ∗
-  DB.db_state kI kR N db.
+  DB.db_state kI kR dbN db.
 
 Definition db_connected' kI kR cs : iProp := ∃ db,
   (compromised_session Init cs ∨ db_client_ready kI kR db) ∗
-  DB.db_state kI kR N db.
+  DB.db_state kI kR dbN db.
 
 Definition db_connected kI kR cs : iProp :=
   RPC.client_connected kI kR cs ∗
@@ -101,10 +101,10 @@ iApply (RPC.client_connected_ok with "conn").
 Qed.
 
 Definition db_mapsto kI kR t1 t2 : iProp :=
-  DB.mapsto kI kR N t1 t2.
+  DB.mapsto kI kR dbN t1 t2.
 
 Definition db_free_at kI kR T : iProp :=
-  DB.free_at kI kR N T.
+  DB.free_at kI kR dbN T.
 
 Lemma db_free_at_diff kI kR T1 T2 :
   T1 ⊆ T2 →
@@ -112,18 +112,18 @@ Lemma db_free_at_diff kI kR T1 T2 :
 Proof. iIntros "%sub". by iApply DB.free_at_diff. Qed.
 
 Lemma client_alloc kI kR E :
-  ↑N.@"client".@kR ⊆ E →
+  ↑dbN.@"client".@kR ⊆ E →
   term_token kI E ={⊤}=∗
   db_disconnected kI kR ∗
   db_free_at kI kR ⊤ ∗
-  term_token kI (E ∖ ↑N.@"client".@kR).
+  term_token kI (E ∖ ↑dbN.@"client".@kR).
 Proof.
 iIntros "%sub kI_token".
 rewrite (term_token_difference _ _ _ sub).
 iDestruct "kI_token" as "[kI_token ?]". iFrame.
-iMod (rep_main_alloc (N := N) kI (kR := kR) [] with "kI_token")
+iMod (rep_main_alloc (N := dbN) kI (kR := kR) [] with "kI_token")
   as "(main & cur & kI_token)"; first solve_ndisj.
-iMod (DB.client_alloc _ (N := N) with "kI_token")
+iMod (DB.client_alloc _ (N := dbN) with "kI_token")
   as "(state & free & kI_token)".
 { solve_ndisj. }
 iModIntro. iFrame. iRight. iExists []. by iFrame.
@@ -163,10 +163,10 @@ Definition server_db_disconnected kI kR vdb : iProp := ∃ db,
   (Conn.failure kI kR ∨ db_server_ready kI kR db).
 
 Lemma server_db_alloc kI kR vdb E :
-  ↑N.@"server".@kI ⊆ E →
+  ↑dbN.@"server".@kI ⊆ E →
   term_token kR E -∗
   SAList.is_alist vdb ∅ ==∗
-  term_token kR (E ∖ ↑N.@"server".@kI) ∗
+  term_token kR (E ∖ ↑dbN.@"server".@kI) ∗
   server_db_disconnected kI kR vdb.
 Proof.
 iIntros "%sub token vdb".
@@ -180,19 +180,19 @@ Definition server ss : iProp := ∃ accounts E,
   sign_key (ss_key ss) ∗
   SAList.is_alist (ss_clients ss) (repr <$> accounts) ∗
   term_token (ss_key ss) E ∗
-  ⌜∀ kI, TKey Open kI ∉ dom accounts → ↑N.@"server".@kI ⊆ E⌝ ∗
+  ⌜∀ kI, TKey Open kI ∉ dom accounts → ↑dbN.@"server".@kI ⊆ E⌝ ∗
   [∗ map] vkI ↦ scs ∈ accounts, ∃ kI, ⌜vkI = TKey Open kI⌝ ∗
      is_lock (scs_name scs) (scs_lock scs)
        (server_db_disconnected kI (ss_key ss) (scs_db scs)).
 
 Lemma serverI kR vclients :
-  term_token kR (↑N.@"server") -∗
+  term_token kR (↑dbN.@"server") -∗
   sign_key kR -∗
   SAList.is_alist vclients ∅ -∗
   server {| ss_key := kR; ss_clients := vclients |}.
 Proof.
 iIntros "token #p_vk clients".
-iExists ∅, (↑N.@"server") => /=.
+iExists ∅, (↑dbN.@"server") => /=.
 iFrame. iSplit => //. iSplit => //.
 iPureIntro. move=> *. solve_ndisj.
 Qed.
@@ -200,10 +200,10 @@ Qed.
 Definition store_call_pred kI kR si ts : iProp :=
   ∃ t1 t2 os,
     ⌜ts = [t1; t2]⌝ ∗
-    rep_update kI kR N [] os (os ++ [Store t1 t2]).
+    rep_update kI kR dbN [] os (os ++ [Store t1 t2]).
 
 Definition store_resp_pred kI kR si ts : iProp :=
-  ∃ os, rep_current kI kR N [] os.
+  ∃ os, rep_current kI kR dbN [] os.
 
 (* MOVE *)
 Lemma to_db_app os o  :
@@ -256,10 +256,10 @@ Qed.
 
 Definition create_call_pred kI kR si ts : iProp :=
   ∃ t1 t2 os, ⌜ts = [t1; t2]⌝ ∗ ⌜DB.to_db os !! t1 = None⌝ ∗
-    rep_update kI kR N [] os (os ++ [Create t1 t2]).
+    rep_update kI kR dbN [] os (os ++ [Create t1 t2]).
 
 Definition create_resp_pred kI kR si ts : iProp :=
-  ∃ os, rep_current kI kR N [] os.
+  ∃ os, rep_current kI kR dbN [] os.
 
 Lemma create_call t1 t2 kI kR cs :
   let P := compromised_session Init cs in
@@ -306,11 +306,11 @@ Qed.
 
 Definition load_call_pred kI kR si ts : iProp :=
   ∃ t1 t2 os, ⌜ts = [t1]⌝ ∗ ⌜DB.to_db os !! t1 = Some t2⌝ ∗
-              rep_update kI kR N [] os (os ++ [Load t1]).
+              rep_update kI kR dbN [] os (os ++ [Load t1]).
 
 Definition load_resp_pred kI kR si ts : iProp :=
   ∃ t1 t2 os, ⌜ts = [t2]⌝ ∗ ⌜DB.to_db os !! t1 = Some t2⌝ ∗
-              rep_current kI kR N [] (os ++ [Load t1]).
+              rep_current kI kR dbN [] (os ++ [Load t1]).
 
 Lemma load_call t1 t2 kI kR cs :
   let P := compromised_session Init cs in
@@ -362,18 +362,19 @@ iSplitL "ready"; iRight.
 Qed.
 
 Definition store_ctx : iProp :=
-  RPC.rpc_pred N "store" store_call_pred store_resp_pred ∗
-  RPC.rpc_pred N "load" load_call_pred load_resp_pred ∗
-  RPC.rpc_pred N "create" create_call_pred create_resp_pred ∗
-  RPC.ctx N.
+  RPC.rpc_pred dbN "store" store_call_pred store_resp_pred ∗
+  RPC.rpc_pred dbN "load" load_call_pred load_resp_pred ∗
+  RPC.rpc_pred dbN "create" create_call_pred create_resp_pred ∗
+  RPC.ctx.
 
 Lemma store_ctx_alloc E :
-  ↑N ⊆ E →
-  seal_pred_token E ==∗
-  store_ctx ∗ seal_pred_token (E ∖ ↑N).
+  ↑dbN ⊆ E →
+  seal_pred_token E -∗
+  RPC.ctx ==∗
+  store_ctx ∗ seal_pred_token (E ∖ ↑dbN).
 Proof.
-iIntros "%sub token".
-rewrite (seal_pred_token_difference (↑N)) => //.
+iIntros "%sub token #?".
+rewrite (seal_pred_token_difference (↑dbN)) => //.
 iDestruct "token" as "[token ?]". iFrame.
 iMod (RPC.rpc_pred_set _ (s := "store") with "token")
   as "[store token]"; try solve_ndisj.
@@ -383,9 +384,6 @@ iMod (RPC.rpc_pred_set _ (s := "load") with "token")
 iFrame.
 iMod (RPC.rpc_pred_set _ (s := "create") with "token")
   as "[create token]"; try solve_ndisj.
-iFrame.
-iMod (RPC.ctx_alloc (N := N) with "token")
-  as "(#? & ?)"; try solve_ndisj.
 Qed.
 
 Ltac solve_ctx :=
@@ -397,20 +395,20 @@ Ltac solve_ctx :=
 
 Lemma store_ctx_store :
   store_ctx -∗
-  RPC.rpc_pred N "store" store_call_pred store_resp_pred.
+  RPC.rpc_pred dbN "store" store_call_pred store_resp_pred.
 Proof. solve_ctx. Qed.
 
 Lemma store_ctx_load :
   store_ctx -∗
-  RPC.rpc_pred N "load" load_call_pred load_resp_pred.
+  RPC.rpc_pred dbN "load" load_call_pred load_resp_pred.
 Proof. solve_ctx. Qed.
 
 Lemma store_ctx_create :
   store_ctx -∗
-  RPC.rpc_pred N "create" create_call_pred create_resp_pred.
+  RPC.rpc_pred dbN "create" create_call_pred create_resp_pred.
 Proof. solve_ctx. Qed.
 
-Lemma store_ctx_rpc_ctx : store_ctx -∗ RPC.ctx N.
+Lemma store_ctx_rpc_ctx : store_ctx -∗ RPC.ctx.
 Proof. solve_ctx. Qed.
 
 End Defs.
