store/client_proofs/load.v
@@ -26,25 +26,23 @@ Implicit Types n : nat.
 Implicit Types γ : gname.
 Implicit Types v : val.
 
-Variable N : namespace.
-
 Lemma wp_client_load c kI kR cs t1 t2 :
   channel c -∗
   cryptis_ctx -∗
-  store_ctx N -∗
+  store_ctx -∗
   public t1 -∗
-  {{{ db_connected N kI kR cs ∗
-      db_mapsto N kI kR t1 t2 }}}
-    Client.load N c (repr cs) t1
+  {{{ db_connected kI kR cs ∗
+      db_mapsto kI kR t1 t2 }}}
+    Client.load c (repr cs) t1
   {{{ t2', RET (repr t2');
-      db_connected N kI kR cs ∗
-      db_mapsto N kI kR t1 t2 ∗
+      db_connected kI kR cs ∗
+      db_mapsto kI kR t1 t2 ∗
       public t2' ∗
       (compromised_session Init cs ∨ ⌜t2' = t2⌝) }}}.
 Proof.
 iIntros "#chan_c #? #ctx #p_t1 !> %Φ [client mapsto] post".
 iDestruct "client" as "(conn & db)".
-iMod (load_call _ t1 with "db mapsto") as "(load & mapsto & waiting)".
+iMod (load_call t1 with "db mapsto") as "(load & mapsto & waiting)".
 wp_lam; wp_pures. wp_list.
 iDestruct "ctx" as "(_ & ? & _ & ctx)".
 wp_apply (RPC.wp_call with "[$conn $load]").
