store/client_proofs/store.v
@@ -25,21 +25,19 @@ Implicit Types n : nat.
 Implicit Types γ : gname.
 Implicit Types v : val.
 
-Variable N : namespace.
-
 Lemma wp_client_store c kI kR cs t1 t2 t2' :
   channel c -∗
   cryptis_ctx -∗
-  store_ctx N -∗
+  store_ctx -∗
   public t1 -∗
   public t2' -∗
-  {{{ db_connected N kI kR cs ∗ db_mapsto N kI kR t1 t2 }}}
-    Client.store N c (repr cs) t1 t2'
-  {{{ RET #(); db_connected N kI kR cs ∗ db_mapsto N kI kR t1 t2' }}}.
+  {{{ db_connected kI kR cs ∗ db_mapsto kI kR t1 t2 }}}
+    Client.store c (repr cs) t1 t2'
+  {{{ RET #(); db_connected kI kR cs ∗ db_mapsto kI kR t1 t2' }}}.
 Proof.
 iIntros "#chan_c #? #ctx #p_t1 #p_t2 !> %Φ [client mapsto] post".
 iDestruct "client" as "(conn & db)".
-iMod (store_call _ t2' with "db mapsto") as "(store & mapsto & waiting)".
+iMod (store_call t2' with "db mapsto") as "(store & mapsto & waiting)".
 wp_lam. wp_pures. wp_list.
 iPoseProof (store_ctx_store with "[//]") as "?".
 iPoseProof (store_ctx_rpc_ctx with "[//]") as "?".
